thys/LLL_Basis_Reduction/Gram_Schmidt_2.thy
@@ -2737,7 +2737,8 @@ next
 qed
 
 
-
+lemma max_list_Max: "ls \<noteq> [] \<Longrightarrow> max_list ls = Max (set ls)"
+  by (induction ls) (auto simp add: max_list_Cons)
 
 section \<open>Bounds\<close>
 
@@ -2746,8 +2747,7 @@ begin
 
 definition "A = Max (sq_norm ` set fs)"
 
-lemma max_list_Max: "ls \<noteq> [] \<Longrightarrow> max_list ls = Max (set ls)"
-  by (induction ls) (auto simp add: max_list_Cons)
+
 
 lemma A_ge_0:
   assumes "0 < m"
@@ -2891,7 +2891,7 @@ abbreviation (input) m where "m \<equiv> length fs_init"
 sublocale gs: gram_schmidt_fs n "TYPE(rat)" "RAT fs_init" .
 
 definition d :: "int vec list \<Rightarrow> nat \<Rightarrow> int" where "d fs k = gs.Gramian_determinant fs k"
-definition D :: "int vec list \<Rightarrow> nat" where "D fs = nat (\<Prod> i < m. d fs i)" 
+definition D :: "int vec list \<Rightarrow> nat" where "D fs = nat (\<Prod> i < length fs. d fs i)" 
 
 lemma of_int_Gramian_determinant:
   assumes "k \<le> length F" "\<And>i. i < length F \<Longrightarrow> dim_vec (F ! i) = n"
